see uneq_cons version

Terms.v
@@ -46,12 +46,18 @@ Fixpoint Union_app (ts : term) (g : Prop) (x : term) : term :=
   | ts => Union []
   end.
 
+Fixpoint disjunct (gvs : list (Prop * term)) : Prop :=
+  match gvs with
+  | [] => False
+  | ((g, _) :: gvs) => g \/ disjunct gvs
+  end.
+
 Inductive empty_union : term -> Prop :=
 | empty_union_nil: empty_union (Union [])
-| empty_union_cons_empty: forall (t ts : term) (g : Prop),
-    empty_union t -> empty_union ts -> empty_union (Union_app ts g t)
-| empty_union_cons_false_guard: forall (t ts : term) (g : Prop),
-    ~ g -> empty_union ts -> empty_union (Union_app ts g t)
+| empty_union_cons_empty: forall (g : Prop) (t : term) (ts : list (Prop * term)),
+    empty_union t -> empty_union (Union ts) -> empty_union (Union ((g, t) :: ts))
+| empty_union_cons_false_guard: forall (g : Prop) (t : term) (ts : list (Prop * term)),
+    ~ g -> empty_union (Union ts) -> empty_union (Union ((g, t) :: ts))
 .
 
 Lemma empty_union_not_theory : forall (t : th), ~ empty_union (Theory t).
@@ -61,53 +67,93 @@ Lemma empty_union_not_location : forall (l : loc), ~ empty_union (Location l).
 Proof. unfold not. intros. inversion H; induction ts; inversion H0. Qed.
 
 Reserved Notation "x =s= y" (at level 50).
+Reserved Notation "x =u= y" (at level 50).
 
 Inductive semantically_equal : relation term :=
 (*| semeq_th : forall (th1 th2 : th), th1 = th2 -> Theory th1 =s= Theory th2
 | semeq_loc : forall (loc1 loc2 : loc), loc1 = loc2 -> Location loc1 =s= Location loc2*)
 (*| semeq_symm : forall (t1 t2 : term), t1 =s= t2 -> t2 =s= t1*)
-| semeq_unionr : forall (t : term) (l : list (Prop * term)), union_equal empty_union t (Union l) -> t =s= Union l
-| semeq_unionl : forall (t : term) (l : list (Prop * term)), union_equal empty_union t (Union l) -> Union l =s= t
+| semeq_unionr : forall (t : term) (l : list (Prop * term)), t =u= Union l -> t =s= Union l
+| semeq_unionl : forall (t : term) (l : list (Prop * term)), t =u= Union l -> Union l =s= t
 | semeq_eq : forall (t1 t2 : term), t1 = t2 -> t1 =s= t2
 where "x =s= y" := (semantically_equal x y)
 with union_equal : (term -> Prop) -> relation term :=
 | uneq_nil : forall (isempty : term -> Prop) (x : term), isempty x -> union_equal isempty x (Union [])
-| uneq_cons_false : forall (isempty : term -> Prop) (x v : term) (g : Prop) (gvs : list (Prop * term)),
-  ~ g -> union_equal isempty x (Union gvs) -> union_equal isempty x (Union ((g, v) :: gvs))
-| uneq_cons_true : forall (isempty : term -> Prop) (x v : term) (g : Prop) (gvs : list (Prop * term)),
-  g -> x =s= v -> union_equal (fun _ => True) x (Union gvs) -> union_equal isempty x (Union ((g, v) :: gvs))
+| uneq_cons : forall (isempty : term -> Prop) (x v : term) (g : Prop) (gvs : list (Prop * term)),
+  (g \/ disjunct gvs) /\
+  ((~ g -> union_equal isempty x (Union gvs)) \/
+   (g -> x =s= v /\ union_equal (fun _ => True) x (Union gvs))) -> union_equal isempty x (Union ((g, v) :: gvs))
+where "x =u= y" := (union_equal empty_union x y)
 .
 
 Lemma empty_test : forall (x : term), Union [] =s= Union [(False, x)].
-Proof. intro x. repeat constructor. tauto. Qed.
+Proof. intro x. apply semeq_unionl. constructor. apply empty_union_cons_false_guard. tauto. constructor. Qed.
+
+
+
 
 
 (* ----------------------------------Relation lemmas-------------------------------------- *)
 Instance union_equal_empty_is_reflexive : Reflexive (union_equal empty_union).
 Proof. unfold Reflexive. intro x. admit. Admitted.
 
-
 Instance semeq_is_reflexive : Reflexive semantically_equal.
 Proof. unfold Reflexive. intro x. destruct x; try repeat constructor. reflexivity. Qed.
 
+Instance unino_equal_empty_is_symmetric : Symmetric (union_equal empty_union).
+Proof. unfold Symmetric. intros x y Hxy. admit. Admitted.
+  
+Instance semeq_is_symmetric : Symmetric semantically_equal.
+Proof. unfold Symmetric. intros x y Hxy. destruct x; destruct y; inversion_clear Hxy; admit. Admitted.
+
+Instance unino_equal_empty_is_transitive : Transitive (union_equal empty_union).
+Proof. unfold Transitive. intros x y z Hxy Hyz. admit. Admitted.
+
+Instance semeq_is_transitive : Transitive semantically_equal.
+Proof. unfold Transitive. intros x y z Hxy Hyz. destruct x; destruct y; inversion_clear Hxy; admit. Admitted.
+
+
+(* ----------------------------------Technical lemmas-------------------------------------- *)
+Lemma union_Uequal_split : forall (gvs1 gvs2 : list (Prop * term)),
+  Union gvs1 =u= Union gvs2 <-> (forall (x : term), x =u= Union gvs1 <-> x =u= Union gvs2).
+Proof. intros gvs1 gvs2. split; intro H.
+  - intro x. split; intro Hg.
+    + symmetry in H. etransitivity; eauto.
+    + etransitivity; eauto.
+  - apply H. reflexivity.
+Qed.
+
+Lemma union_Sequal_split : forall (gvs1 gvs2 : list (Prop * term)),
+  Union gvs1 =s= Union gvs2 <-> (forall (x : term), Union gvs1 =s= x <-> Union gvs2 =s= x).
+Proof. intros gvs1 gvs2. split; intro H.
+  - intro x. split; intro Hg.
+    + symmetry in H. etransitivity; eauto.
+    + etransitivity; eauto.
+  - apply H. reflexivity.
+Qed.
 
 
 (* ----------------------------------Properties lemmas-------------------------------------- *)
 Lemma union_True : forall (t : term), Union [(True, t)] =s= t.
-Proof. intro t. constructor. apply uneq_cons_true.
-  - constructor.
+Proof. intro t. constructor. apply uneq_cons. right. intros _. split.
   - reflexivity.
   - repeat constructor.
 Qed.
 
 Lemma union_false_erasing : forall (t : term) (gvs : list (Prop * term)), Union ((False, t) :: gvs) =s= Union gvs.
-Proof. intros t gvs. apply semeq_unionr. apply uneq_cons_false; auto. reflexivity. Qed.
+Proof. intros t gvs. apply semeq_unionl. apply uneq_cons. left. intros _. reflexivity. Qed.
 
 Lemma union_unfolding : forall (g : Prop) (xgvs ygvs : list (Prop * term)),
   Union ((g, Union xgvs) :: ygvs) =s= Union (map (fun x => match x with (g', v) => (g /\ g', v) end) xgvs ++ ygvs).
 Proof. intros g xgvs ygvs. admit. Admitted.
 
+Lemma union_same_value_lr : forall (g1 g2 : Prop) (v x : term), x =u= Union [(g1, v); (g2, v)] <-> x =u= Union [(g1 \/ g2, v)].
+Proof. admit. Admitted.
+
 Lemma union_same_value : forall (g1 g2 : Prop) (v : term) (gvs : list (Prop * term)),
   Union ((g1, v) :: (g2, v) :: gvs) =s= Union ((g1 \/ g2, v) :: gvs).
 Proof. intros g1 g2 v gvs. induction gvs.
+  - apply union_Sequal_split. intro x. split; intro H; constructor; inversion_clear H;
+    try (subst; apply union_same_value_lr; auto); solve [reflexivity | symmetry; assumption].
   - 
+Qed.
